coq/lang/RuleTree.v
@@ -1,0 +1,84 @@
+Set Implicit Arguments.
+From Lang Require Import Util Nodes RuleGraphs.
+
+Section RuleTree.
+
+  
+Variable univ : universe.
+
+Notation stmt := univ.(stmt).
+Notation valid_stmt := univ.(valid_stmt).
+
+Variable ps : proof_system univ.
+
+Notation rule := ps.(rule).
+Notation liftable := ps.(liftable).
+Notation valid_rule := ps.(valid_rule).
+
+Reserved Notation "conc_of_tree." (at level 80).
+
+(*Inductive rule_tree : Type :=
+  | TLift (conc : stmt) (Hlift : liftable conc)
+  | TRule (conc : stmt) (*(prems : list stmt)*) (tprems : list rule_tree)
+    (*(Hprems : )*)
+    (r : rule) (Hval : valid_rule r conc (List.map (conc_of_tree.) tprems))
+where
+  "conc_of_tree." :=
+  (fun (rt : rule_tree) => match rt with
+    | TLift conc _ => conc
+    | TRule conc _ _ _ _ => conc end).
+*)
+
+(*Inductive rule_tree : Prop :=
+  | TLift (conc : stmt) (Hlift : liftable conc) : rule_tree
+  | TRule (conc : stmt) (prems : list stmt)
+    (r : rule) (Hr : valid_rule r prems conc)
+    (Hprems : List.Forall rule_tree prems) : rule_tree conc.
+
+Definition root (rt : rule_tree) :=
+  match rt with
+  | TLift conc _ => conc
+  | TRule conc _ _ _ _ => conc
+  end.
+
+Definition re_root (tprems : List rule_tree) (conc : stmt)
+  ()
+
+
+    (r : rule) (Hprems : valid_rule r (List.map root tprems) conc) :
+    rule_tree_valid (TRule conc tprems r)
+  .*)
+
+Inductive _rule_tree : Type :=
+  | TLift (conc : stmt) 
+  | TRule (conc : stmt) (tprems : list _rule_tree) (r : rule)
+  .
+
+Definition root (rt : _rule_tree) :=
+  match rt with
+  | TLift conc => conc
+  | TRule conc _ _ => conc
+  end.
+
+Inductive rule_tree_valid : _rule_tree -> Prop :=
+  | VTLift (conc : stmt) (Hlift : liftable conc) : rule_tree_valid (TLift conc)
+  | VTRule (conc : stmt) (tprems : list _rule_tree)
+    (r : rule) (Hprems : valid_rule r (List.map root tprems) conc) :
+    rule_tree_valid (TRule conc tprems r)
+  .
+
+Definition rule_tree := { rt : _rule_tree | rule_tree_valid rt }.
+Notation get_tree := (@proj1_sig _rule_tree rule_tree_valid).
+
+Definition re_root (conc : stmt) (tprems : list rule_tree) (r : rule)
+  (Hprems : valid_rule r (List.map (root ∘ get_tree) tprems) conc) : rule_tree.
+pose (TRule conc (List.map get_tree tprems) r) as _rt.
+assert (rule_tree_valid _rt).
+2: { refine (exist _ _ H). }
+apply VTRule. now rewrite List.map_map.
+Defined.
+
+
+
+
+End RuleTree.
